Add rip, eip, ip registers

src/Assembly/Syntax.v
@@ -18,9 +18,9 @@ Local Set Implicit Arguments.
 Local Set Primitive Projections.
 
 Inductive REG :=
-|     rax |     rcx |     rdx |     rbx | rsp  | rbp  | rsi  | rdi  | r8  | r9  | r10  | r11  | r12  | r13  | r14  | r15
-|     eax |     ecx |     edx |     ebx | esp  | ebp  | esi  | edi  | r8d | r9d | r10d | r11d | r12d | r13d | r14d | r15d
-|      ax |      cx |      dx |      bx |  sp  |  bp  |  si  |  di  | r8w | r9w | r10w | r11w | r12w | r13w | r14w | r15w
+|     rax |     rcx |     rdx |     rbx | rsp  | rbp  | rsi  | rdi  | r8  | r9  | r10  | r11  | r12  | r13  | r14  | r15  | rip
+|     eax |     ecx |     edx |     ebx | esp  | ebp  | esi  | edi  | r8d | r9d | r10d | r11d | r12d | r13d | r14d | r15d | eip
+|      ax |      cx |      dx |      bx |  sp  |  bp  |  si  |  di  | r8w | r9w | r10w | r11w | r12w | r13w | r14w | r15w | ip
 | ah | al | ch | cl | dh | dl | bh | bl |  spl |  bpl |  sil |  dil | r8b | r9b | r10b | r11b | r12b | r13b | r14b | r15b
 .
 
@@ -212,11 +212,11 @@ Definition Lines := list Line.
 
 Definition reg_size (r : REG) : N :=
       match r with
-      |(    rax |     rcx |     rdx |     rbx | rsp  | rbp  | rsi  | rdi  | r8  | r9  | r10  | r11  | r12  | r13  | r14  | r15 )
+      |(    rax |     rcx |     rdx |     rbx | rsp  | rbp  | rsi  | rdi  | r8  | r9  | r10  | r11  | r12  | r13  | r14  | r15  | rip)
        => 64
-      |(    eax |     ecx |     edx |     ebx | esp  | ebp  | esi  | edi  | r8d | r9d | r10d | r11d | r12d | r13d | r14d | r15d)
+      |(    eax |     ecx |     edx |     ebx | esp  | ebp  | esi  | edi  | r8d | r9d | r10d | r11d | r12d | r13d | r14d | r15d | eip)
        => 32
-      |(     ax |      cx |      dx |      bx |  sp  |  bp  |  si  |  di  | r8w | r9w | r10w | r11w | r12w | r13w | r14w | r15w)
+      |(     ax |      cx |      dx |      bx |  sp  |  bp  |  si  |  di  | r8w | r9w | r10w | r11w | r12w | r13w | r14w | r15w | ip)
        => 16
       |(ah | al | ch | cl | dh | dl | bh | bl |  spl |  bpl |  sil |  dil | r8b | r9b | r10b | r11b | r12b | r13b | r14b | r15b)
        => 8
@@ -290,6 +290,7 @@ Definition widest_register_of (r : REG) : REG :=
   | (r13b | r13w | r13d | r13) => r13
   | (r14b | r14w | r14d | r14) => r14
   | (r15b | r15w | r15d | r15) => r15
+  | (ip | eip | rip) => rip
   end.
 
 Definition widest_registers := Eval lazy in List.filter (fun x => REG_beq x (widest_register_of x)) (list_all REG).
